kill admit

src/lib/kuiper/Kuiper.Approximates.fst
@@ -4,6 +4,15 @@ open Kuiper
 open FStar.Real
 open Kuiper.Scalars
 
+let to_real_seq_is_approx (#a:Type) {| scalar a, d : real_like a |}
+  (s : seq a)
+  : Lemma (seq_approximates s (to_real_seq s))
+          [SMTPat (seq_approximates s (to_real_seq s))]
+  = let aux (x : a) : Lemma (x `approximates` to_real x)
+      = d.to_real_ok x
+    in
+    Classical.forall_intro aux
+
 let real_seq_sum_append
   (r1 r2 : seq Real.real)
   : Lemma (ensures real_seq_sum (r1 `Seq.append` r2) == real_seq_sum r1 +. real_seq_sum r2)
